Cardinal addition
Signed-off-by: zeramorphic <zeramorphic@proton.me>

ConNF/External/Basic.lean
@@ -20,6 +20,13 @@ namespace ConNF
 variable [Params.{u}] {α β γ δ ε ζ : Λ} (hβ : (β : TypeIndex) < α) (hγ : (γ : TypeIndex) < β)
   (hδ : (δ : TypeIndex) < γ) (hε : (ε : TypeIndex) < δ) (hζ : (ζ : TypeIndex) < ε)
 
+theorem inter_comm (x y : TSet α) :
+    x ⊓' y = y ⊓' x := by
+  apply ext hβ
+  intro z
+  rw [mem_inter_iff, mem_inter_iff]
+  exact And.comm
+
 def union (x y : TSet α) : TSet α :=
   (xᶜ' ⊓' yᶜ')ᶜ'
 
@@ -33,18 +40,46 @@ theorem mem_union_iff (x y : TSet α) :
   intro z
   rw [mem_compl_iff, mem_inter_iff, mem_compl_iff, mem_compl_iff, or_iff_not_and_not]
 
+def symmDiff (x y : TSet α) : TSet α :=
+  (x ⊓' yᶜ') ⊔' (xᶜ' ⊓' y)
+
+notation:100 x:100 " ∆[" h "] " y:100 => _root_.ConNF.symmDiff h x y
+notation:100 x:100 " ∆' " y:100 => x ∆[by assumption] y
+
+@[simp]
+theorem mem_symmDiff_iff (x y : TSet α) :
+    ∀ z : TSet β, z ∈' x ∆' y ↔ (z ∈' x ↔ ¬(z ∈' y)) := by
+  rw [symmDiff]
+  intro z
+  simp only [mem_union_iff, mem_inter_iff, mem_compl_iff]
+  tauto
+
+def diff (x y : TSet α) : TSet α :=
+  x ⊓' yᶜ'
+
+notation:70 x:70 " \\[" h "] " y:70 => _root_.ConNF.diff h x y
+notation:70 x:70 " \\' " y:70 => x \[by assumption] y
+
+@[simp]
+theorem mem_diff_iff (x y : TSet α) :
+    ∀ z : TSet β, z ∈' x \' y ↔ z ∈' x ∧ ¬(z ∈' y) := by
+  rw [diff]
+  intro z
+  simp only [mem_union_iff, mem_inter_iff, mem_compl_iff]
+
 def higherIndex (α : Λ) : Λ :=
   (exists_gt α).choose
 
-theorem lt_higherIndex {α : Λ} :
+/-- A short name is chosen because of its frequency of use. -/
+theorem high {α : Λ} :
     (α : TypeIndex) < higherIndex α :=
   WithBot.coe_lt_coe.mpr (exists_gt α).choose_spec
 
 theorem tSet_nonempty (h : ∃ β : Λ, (β : TypeIndex) < α) : Nonempty (TSet α) := by
   obtain ⟨α', hα⟩ := h
   constructor
-  apply typeLower lt_higherIndex lt_higherIndex lt_higherIndex hα
-  apply cardinalOne lt_higherIndex lt_higherIndex
+  apply typeLower high high high hα
+  apply cardinalOne high high
 
 def empty : TSet α :=
   (tSet_nonempty ⟨β, hβ⟩).some ⊓' (tSet_nonempty ⟨β, hβ⟩).someᶜ'
@@ -72,7 +107,7 @@ def orderedPairs : TSet α :=
 @[simp]
 theorem mem_orderedPairs_iff (x : TSet β) :
     x ∈' orderedPairs hβ hγ hδ ↔ ∃ a b, x = ⟨a, b⟩' := by
-  simp only [orderedPairs, vCross_spec, mem_univ_iff, and_true]
+  simp only [orderedPairs, mem_vCross_iff, mem_univ_iff, and_true]
 
 def converse (x : TSet α) : TSet α :=
   converse' hβ hγ hδ x ⊓' orderedPairs hβ hγ hδ
@@ -91,14 +126,14 @@ def cross (x y : TSet γ) : TSet α :=
 theorem mem_cross_iff (x y : TSet γ) :
     ∀ a, a ∈' cross hβ hγ hδ x y ↔ ∃ b c, a = ⟨b, c⟩' ∧ b ∈' x ∧ c ∈' y := by
   intro a
-  rw [cross, mem_inter_iff, vCross_spec]
+  rw [cross, mem_inter_iff, mem_vCross_iff]
   constructor
   · rintro ⟨h₁, b, c, rfl, h₂⟩
-    simp only [op_mem_converse_iff, vCross_spec, op_inj] at h₁
+    simp only [op_mem_converse_iff, mem_vCross_iff, op_inj] at h₁
     obtain ⟨b', c', ⟨rfl, rfl⟩, h₁⟩ := h₁
     exact ⟨b, c, rfl, h₁, h₂⟩
   · rintro ⟨b, c, rfl, h₁, h₂⟩
-    simp only [op_mem_converse_iff, vCross_spec, op_inj]
+    simp only [op_mem_converse_iff, mem_vCross_iff, op_inj]
     exact ⟨⟨c, b, ⟨rfl, rfl⟩, h₁⟩, ⟨b, c, ⟨rfl, rfl⟩, h₂⟩⟩
 
 def singletonImage (x : TSet β) : TSet α :=
@@ -134,7 +169,7 @@ theorem externalRel_converse (r : TSet α) :
 
 /-- The codomain of a relation. -/
 def codom (r : TSet α) : TSet γ :=
-  (typeLower lt_higherIndex hβ hγ hδ (singletonImage lt_higherIndex hβ hγ hδ r)ᶜ[lt_higherIndex])ᶜ'
+  (typeLower high hβ hγ hδ (singletonImage high hβ hγ hδ r)ᶜ[high])ᶜ'
 
 @[simp]
 theorem mem_codom_iff (r : TSet α) (x : TSet δ) :
@@ -142,7 +177,7 @@ theorem mem_codom_iff (r : TSet α) (x : TSet δ) :
   simp only [codom, mem_compl_iff, mem_typeLower_iff, not_forall, not_not]
   constructor
   · rintro ⟨y, hy⟩
-    obtain ⟨a, b, rfl, hb⟩ := exists_of_mem_singletonImage lt_higherIndex hβ hγ hδ hy
+    obtain ⟨a, b, rfl, hb⟩ := exists_of_mem_singletonImage high hβ hγ hδ hy
     rw [singleton_inj] at hb
     subst hb
     rw [singletonImage_spec] at hy
@@ -180,6 +215,18 @@ theorem subset_spec :
   simp only [subset, mem_inter_iff, subset'_spec, mem_orderedPairs_iff, op_inj, exists_and_left,
     exists_eq', and_true]
 
+@[simp]
+theorem singleton_subset_iff (a : TSet β) (b : TSet α) :
+    {a}' ⊆[TSet β] b ↔ a ∈' b := by
+  constructor
+  · intro h
+    apply h a
+    rw [typedMem_singleton_iff']
+  · intro h x hx
+    rw [typedMem_singleton_iff'] at hx
+    cases hx
+    exact h
+
 def membership : TSet α :=
   subset hβ hγ hδ hε ⊓' cross hβ hγ hδ (cardinalOne hδ hε) (univ hδ)
 
@@ -199,9 +246,9 @@ theorem membership_spec :
     exact h
 
 def powerset (x : TSet β) : TSet α :=
-  dom lt_higherIndex lt_higherIndex hβ
-    (subset lt_higherIndex lt_higherIndex hβ hγ ⊓[lt_higherIndex]
-      vCross lt_higherIndex lt_higherIndex hβ {x}')
+  dom high high hβ
+    (subset high high hβ hγ ⊓[high]
+      vCross high high hβ {x}')
 
 @[simp]
 theorem mem_powerset_iff (x y : TSet β) :
@@ -209,25 +256,25 @@ theorem mem_powerset_iff (x y : TSet β) :
   rw [powerset, mem_dom_iff]
   constructor
   · rintro ⟨z, h⟩
-    simp only [ExternalRel, mem_inter_iff, subset_spec, vCross_spec, op_inj,
+    simp only [ExternalRel, mem_inter_iff, subset_spec, mem_vCross_iff, op_inj,
       typedMem_singleton_iff', exists_eq_right, exists_and_right, exists_eq', true_and] at h
     cases h.2
     exact h.1
   · intro h
     refine ⟨y, ?_⟩
-    simp only [ExternalRel, mem_inter_iff, subset_spec, h, vCross_spec, op_inj,
+    simp only [ExternalRel, mem_inter_iff, subset_spec, h, mem_vCross_iff, op_inj,
       typedMem_singleton_iff', exists_eq_right, and_true, exists_eq', and_self]
 
 /-- The set `ι²''x = {{{a}} | a ∈ x}`. -/
-def doubleSingleton (x : TSet γ) : TSet α :=
+def doubleSingletons (x : TSet γ) : TSet α :=
   cross hβ hγ hδ x x ⊓' cardinalOne hβ hγ
 
 @[simp]
-theorem mem_doubleSingleton_iff (x : TSet γ) :
-    ∀ y : TSet β, y ∈' doubleSingleton hβ hγ hδ x ↔
+theorem mem_doubleSingletons_iff (x : TSet γ) :
+    ∀ y : TSet β, y ∈' doubleSingletons hβ hγ hδ x ↔
     ∃ z : TSet δ, z ∈' x ∧ y = { {z}' }' := by
   intro y
-  rw [doubleSingleton, mem_inter_iff, mem_cross_iff, mem_cardinalOne_iff]
+  rw [doubleSingletons, mem_inter_iff, mem_cross_iff, mem_cardinalOne_iff]
   constructor
   · rintro ⟨⟨b, c, h₁, h₂, h₃⟩, ⟨a, rfl⟩⟩
     obtain ⟨hbc, rfl⟩ := (op_eq_singleton_iff _ _ _ _ _).mp h₁.symm
@@ -239,16 +286,17 @@ theorem mem_doubleSingleton_iff (x : TSet γ) :
       tauto
     · exact ⟨_, rfl⟩
 
-/-- The union of a set of *singletons*: `ι⁻¹''x = {a | {a} ∈ x}`. -/
+/-- The union of a set of *singletons*: `ι⁻¹''x = {a | {a} ∈ x}`.
+Scott Fenton calls this the "unit union". -/
 def singletonUnion (x : TSet α) : TSet β :=
-  typeLower lt_higherIndex lt_higherIndex hβ hγ
-    (vCross lt_higherIndex lt_higherIndex hβ x)
+  typeLower high high hβ hγ
+    (vCross high high hβ x)
 
 @[simp]
 theorem mem_singletonUnion_iff (x : TSet α) :
     ∀ y : TSet γ, y ∈' singletonUnion hβ hγ x ↔ {y}' ∈' x := by
   intro y
-  simp only [singletonUnion, mem_typeLower_iff, vCross_spec, op_inj]
+  simp only [singletonUnion, mem_typeLower_iff, mem_vCross_iff, op_inj]
   constructor
   · intro h
     obtain ⟨a, b, ⟨rfl, rfl⟩, hy⟩ := h {y}'
@@ -256,22 +304,33 @@ theorem mem_singletonUnion_iff (x : TSet α) :
   · intro h b
     exact ⟨b, _, ⟨rfl, rfl⟩, h⟩
 
+/-- The set of singletons of a set: `ι''x = {{a} | a ∈ x}`.
+Scott Fenton calls this the "unit powerset". -/
+def singletons (x : TSet β) : TSet α :=
+  singletonUnion high hβ (doubleSingletons high hβ hγ x)
+
+@[simp]
+theorem mem_singletons_iff (x : TSet β) :
+    ∀ y : TSet β, y ∈' singletons hβ hγ x ↔ ∃ t : TSet γ, t ∈' x ∧ y = {t}' := by
+  intro y
+  simp only [singletons, mem_singletonUnion_iff, mem_doubleSingletons_iff, singleton_inj]
+
 /--
 The union of a set of sets.
 
 ```
-singletonUnion dom {⟨{a}, b⟩ | a ∈ b} ∩ (1 × x) =
-singletonUnion dom {⟨{a}, b⟩ | a ∈ b ∧ b ∈ x} =
-singletonUnion {{a} | a ∈ b ∧ b ∈ x} =
+⋃ x =
 {a | a ∈ b ∧ b ∈ x} =
-⋃ x
+singletonUnion {{a} | a ∈ b ∧ b ∈ x} =
+singletonUnion dom {⟨{a}, b⟩ | a ∈ b ∧ b ∈ x} =
+singletonUnion dom ({⟨{a}, b⟩ | a ∈ b} ∩ (1 × x))
 ```
 -/
 def sUnion (x : TSet α) : TSet β :=
-  singletonUnion hβ hγ
-    (dom lt_higherIndex lt_higherIndex hβ
-      (membership lt_higherIndex lt_higherIndex hβ hγ ⊓[lt_higherIndex]
-        cross lt_higherIndex lt_higherIndex hβ (cardinalOne hβ hγ) x))
+  singletonUnion hβ hγ <|
+  dom high high hβ <|
+  membership high high hβ hγ ⊓[high]
+    cross high high hβ (cardinalOne hβ hγ) x
 
 @[simp]
 theorem mem_sUnion_iff (x : TSet α) :
@@ -286,6 +345,65 @@ theorem mem_sUnion_iff (x : TSet α) :
     exact ⟨z, h₃, h₁⟩
   · rintro ⟨z, h₂, h₃⟩
     exact ⟨z, h₃, _, _, ⟨rfl, rfl⟩, ⟨y, rfl⟩, h₂⟩
+
+/-- The set of all ordered triples. -/
+def orderedTriples : TSet α :=
+  cross hβ hγ hδ (doubleSingletons hδ hε hζ (univ hζ)) (vCross hδ hε hζ (univ hζ))
+
+@[simp]
+theorem mem_orderedTriples_iff (x : TSet β) :
+    x ∈' orderedTriples hβ hγ hδ hε hζ ↔ ∃ a b c, x = ⟨ { {a}' }', ⟨b, c⟩' ⟩' := by
+  simp only [orderedTriples, mem_cross_iff, mem_doubleSingletons_iff, mem_univ_iff, true_and,
+    mem_vCross_iff, and_true]
+  constructor
+  · rintro ⟨_, _, rfl, ⟨a, rfl⟩, ⟨b, c, rfl⟩⟩
+    exact ⟨_, _, _, rfl⟩
+  · rintro ⟨a, b, c, rfl⟩
+    exact ⟨_, _, rfl, ⟨_, rfl⟩, ⟨_, _, rfl⟩⟩
+
+def insertion2 (x : TSet γ) : TSet α :=
+  insertion2' hβ hγ hδ hε hζ x ⊓' orderedTriples hβ hγ hδ hε hζ
+
+@[simp]
+theorem insertion2_spec (x : TSet γ) :
+    ∀ a b c, ⟨ { {a}' }', ⟨b, c⟩' ⟩' ∈' insertion2 hβ hγ hδ hε hζ x ↔
+    ⟨a, c⟩' ∈' x := by
+  simp only [insertion2, mem_inter_iff, insertion2'_spec, mem_orderedTriples_iff, op_inj,
+    singleton_inj, exists_and_left, exists_eq', and_true, implies_true]
+
+def insertion3 (x : TSet γ) : TSet α :=
+  insertion3' hβ hγ hδ hε hζ x ⊓' orderedTriples hβ hγ hδ hε hζ
+
+@[simp]
+theorem insertion3_spec (x : TSet γ) :
+    ∀ a b c, ⟨ { {a}' }', ⟨b, c⟩' ⟩' ∈' insertion3 hβ hγ hδ hε hζ x ↔
+    ⟨a, b⟩' ∈' x := by
+  simp only [insertion3, mem_inter_iff, insertion3'_spec, mem_orderedTriples_iff, op_inj,
+    singleton_inj, exists_and_left, exists_eq', and_true, implies_true]
+
+/-- The preimage of a set under a relation. -/
+def preimage (r : TSet α) (x : TSet γ) : TSet γ :=
+  dom hβ hγ hδ (r ⊓' vCross hβ hγ hδ x)
+
+@[simp]
+theorem mem_preimage_iff (r : TSet α) (x : TSet γ) (y : TSet δ) :
+    y ∈' preimage hβ hγ hδ r x ↔ y ∈ (ExternalRel hβ hγ hδ r).preimage {a | a ∈' x} := by
+  simp only [preimage, mem_dom_iff, Rel.dom, ExternalRel, mem_inter_iff, mem_vCross_iff, op_inj,
+    Set.mem_setOf_eq, Rel.preimage, Rel.image, Rel.inv, flip]
+  constructor
+  · rintro ⟨a, h₁, _, _, ⟨rfl, rfl⟩, h₂⟩
+    exact ⟨a, h₂, h₁⟩
+  · rintro ⟨a, h₁, h₂⟩
+    exact ⟨a, h₂, _, _, ⟨rfl, rfl⟩, h₁⟩
+
+/-- The image of a set under a relation. -/
+def image (r : TSet α) (x : TSet γ) : TSet γ :=
+  preimage hβ hγ hδ (converse hβ hγ hδ r) x
+
+@[simp]
+theorem mem_image_iff (r : TSet α) (x : TSet γ) (y : TSet δ) :
+    y ∈' image hβ hγ hδ r x ↔ y ∈ (ExternalRel hβ hγ hδ r).image {a | a ∈' x} := by
+  simp only [image, mem_preimage_iff, externalRel_converse, Rel.preimage_inv]
 
 theorem exists_smallUnion (s : Set (TSet α)) (hs : Small s) :
     ∃ x : TSet α, ∀ y : TSet β, y ∈' x ↔ ∃ t ∈ s, y ∈' t := by
