ConNF/External/Counting.lean
@@ -5,6 +5,9 @@ import ConNF.External.Basic
 
 In this file...
 
+We are roughly following Scott Fenton's development of NF:
+<https://us.metamath.org/nfeuni/mmnf.html>.
+
 ## Main declarations
 
 * `ConNF.foo`: Something new.
@@ -17,12 +20,103 @@ open Cardinal Ordinal ConNF.TSet
 
 namespace ConNF
 
-variable [Params.{u}] {α β γ δ ε ζ : Λ} (hβ : (β : TypeIndex) < α) (hγ : (γ : TypeIndex) < β)
+variable [Params.{u}] {α β γ δ ε ζ η : Λ} (hβ : (β : TypeIndex) < α) (hγ : (γ : TypeIndex) < β)
   (hδ : (δ : TypeIndex) < γ) (hε : (ε : TypeIndex) < δ) (hζ : (ζ : TypeIndex) < ε)
+  (hη : (η : TypeIndex) < ζ)
 
-/-- The set `{z ∪ {a} | z ∈ x}`. -/
-def insert (x : TSet α) : TSet α :=
-  sorry
+-- ((( Ins3k disjoint) ∖
+--   (( Ins2k Ins2k Sk ⊕ ( Ins2k Ins3k Sk ∪ Ins3k SIk SIk Sk )) “k ℘1℘1℘1℘11c)) “k ℘1℘1B) “k A)
+
+-- ( Ins2k Ins2k Sk ⊕ ( Ins2k Ins3k Sk ∪ Ins3k SIk SIk Sk ))
+
+/-- The set `{⟨x, y⟩ | x ∩ y = ∅}` (or rather, a set that contains only these Kuratowski pairs). -/
+def disjoint : TSet α :=
+  (image high high hβ
+    (insertion3 high high hβ hγ hδ (subset hβ hγ hδ hε) ⊓[high]
+      insertion2 high high hβ hγ hδ (subset hβ hγ hδ hε))
+    (singletons hβ hγ (singletons hγ hδ (cardinalOne hδ hε))))ᶜ'
+
+theorem mem_disjoint_iff' (x y : TSet δ) :
+    ⟨x, y⟩' ∈' disjoint hβ hγ hδ hε ↔ ∀ z : TSet ε, ¬z ∈' x ⊓' y := by
+  simp only [disjoint, mem_compl_iff, mem_image_iff, Rel.image, mem_singletons_iff,
+    mem_cardinalOne_iff, Set.mem_setOf_eq, ExternalRel, mem_inter_iff, not_exists, not_and,
+    forall_exists_index, and_imp, forall_eq_apply_imp_iff, insertion3_spec, subset_spec,
+    singleton_subset_iff, insertion2_spec]
+
+@[simp]
+theorem mem_disjoint_iff (x y : TSet δ) :
+    ⟨x, y⟩' ∈' disjoint hβ hγ hδ hε ↔ x ⊓' y = empty hε := by
+  rw [mem_disjoint_iff']
+  constructor
+  · intro h
+    apply ext hε
+    simp only [h, mem_empty_iff, implies_true]
+  · intro h
+    rw [← ext_iff hε] at h
+    simp only [h, mem_empty_iff, not_false_eq_true, implies_true]
+
+/-- The set `{⟨{{z}}, ⟨y, x⟩ | y ∪ z = x}` (or rather, again,
+a set that contains only these pairs). -/
+def unionEq : TSet α :=
+  (image high high hβ
+    (insertion2 high high hβ hγ hδ (insertion2 hβ hγ hδ hε hζ (subset hδ hε hζ hη)) ∆[high]
+      (insertion2 high high hβ hγ hδ (insertion3 hβ hγ hδ hε hζ (subset hδ hε hζ hη)) ⊔[high]
+      insertion3 high high hβ hγ hδ (singletonImage hβ hγ hδ hε
+        (singletonImage hγ hδ hε hζ (subset hδ hε hζ hη)))))
+    (singletons hβ hγ (singletons hγ hδ (singletons hδ hε
+      (singletons hε hζ (cardinalOne hζ hη))))))ᶜ'
+
+theorem mem_unionEq_iff' (x y z : TSet ζ) :
+    ⟨ { {z}' }', ⟨y, x⟩' ⟩[hγ, hδ] ∈' unionEq hβ hγ hδ hε hζ hη ↔
+      ∀ a : TSet η, ¬(a ∈' x ↔ ¬a ∈' y ∧ ¬a ∈' z) := by
+  simp only [unionEq, mem_compl_iff, mem_image_iff, Rel.image, mem_singletons_iff,
+    mem_cardinalOne_iff, Set.mem_setOf_eq, ExternalRel, mem_symmDiff_iff, mem_union_iff, not_or,
+    not_exists, not_and, forall_exists_index, and_imp, forall_eq_apply_imp_iff, insertion2_spec,
+    subset_spec, singleton_subset_iff, insertion3_spec, singletonImage_spec]
+
+@[simp]
+theorem mem_unionEq_iff (x y z : TSet ζ) :
+    ⟨ { {z}' }', ⟨y, x⟩' ⟩[hγ, hδ] ∈' unionEq hβ hγ hδ hε hζ hη ↔ y ⊔' z = x := by
+  rw [mem_unionEq_iff']
+  constructor
+  · intro h
+    apply ext hη
+    intro t
+    rw [mem_union_iff]
+    have := h t
+    rw [iff_comm, not_iff, not_and_or, not_not, not_not] at this
+    exact this
+  · rintro rfl a
+    rw [iff_comm, not_iff, not_and_or, not_not, not_not, mem_union_iff]
+
+/-- The sum of two cardinals: `x + y = {a ∪ b | a ∈ x ∧ b ∈ y ∧ a ∩ b = ∅}`. -/
+def cardAdd (x y : TSet α) : TSet α :=
+  image high high hβ
+    (image high high high
+      (insertion3 high high high high hβ (disjoint high high hβ hγ)
+        ⊓[high] (unionEq high high high high hβ hγ))
+      (singletons high high (singletons high hβ y))) x
+
+@[simp]
+theorem mem_cardAdd_iff (x y : TSet α) (z : TSet β) :
+    z ∈' cardAdd hβ hγ x y ↔
+    ∃ a b : TSet β, a ∈' x ∧ b ∈' y ∧ a ⊓' b = empty hγ ∧ a ⊔' b = z := by
+  simp only [cardAdd, mem_image_iff, Rel.image, Set.mem_setOf_eq, ExternalRel, mem_singletons_iff,
+    mem_inter_iff, exists_and_left]
+  constructor
+  · rintro ⟨a, ha, _, ⟨_, ⟨b, hb, rfl⟩, rfl⟩, h₁, h₂⟩
+    rw [insertion3_spec, mem_disjoint_iff] at h₁
+    rw [mem_unionEq_iff] at h₂
+    cases h₂
+    rw [inter_comm] at h₁
+    exact ⟨a, ha, b, hb, h₁, rfl⟩
+  · rintro ⟨a, ha, b, hb, h, rfl⟩
+    refine ⟨a, ha, _, ⟨_, ⟨b, hb, rfl⟩, rfl⟩, ?_⟩
+    simp only [insertion3_spec, mem_disjoint_iff, mem_unionEq_iff, and_true]
+    rwa [inter_comm]
+
+/-- The successor of a cardinal: `x + 1 = {a ∪ {b} | a ∈ x, b ∉ a}`. -/
+def succ (x : TSet α) : TSet α := sorry
 
 def cardinalNat (n : ℕ) : TSet α :=
   (TSet.exists_cardinalOne hβ hγ).choose
